Most recent reactive theories including ACP + CSP STOP closure, Parallel definitions

theories/theories/utp_acp.thy
@@ -14,22 +14,43 @@ imports
 begin
 
 definition ACP1 :: "'a WF_PREDICATE \<Rightarrow> 'a WF_PREDICATE" where
-"ACP1 P = `P \<and> (($tr =$tr\<acute>) \<Rightarrow> $wait)` "
+"ACP1 P = `P \<and> ( ok \<and> ($tr =$tr\<acute>) \<Rightarrow> $wait\<acute>)` "
+
+syntax 
+  "_upred_ACP1" :: "upred \<Rightarrow> upred" ("ACP1'(_')")
+translations
+  "_upred_ACP1 P" == "CONST ACP1 P"
+
+lemma ACP1_idempotent : "ACP1 (ACP1 P) = ACP1 P" by (simp add:ACP1_def, utp_pred_tac)
+
+lemma ACP1_monotonic : "[P \<Rightarrow> Q] \<Longrightarrow> [ACP1(P) \<Rightarrow> ACP1(Q)]" by(simp add:ACP1_def, utp_pred_auto_tac)
+
+lemma ACP1_R1_commute : "ACP1 (R1 P) = R1 (ACP1 P)" by (simp add:ACP1_def, utp_pred_auto_tac)
+lemma ACP1_R2_commute : "ACP1 (R2 P) = R2 (ACP1 P)" 
+proof -
+have "R2 (ACP1 P) = `R2(P) \<and> (ok \<and> \<langle>\<rangle> = ($tr\<acute> - $tr) \<Rightarrow> $wait\<acute>)`"by(simp add:ACP1_def R2_def R2s_def usubst typing defined closure, utp_pred_auto_tac)
+also have "... = `R2(P) \<and> (ok \<and> ($tr = $tr\<acute>) \<Rightarrow> $wait\<acute>)`"by(simp add: helper4, utp_pred_auto_tac)
+finally show ?thesis by(simp add:ACP1_def) 
+qed
+
+lemma ACP1_R3_commute : "ACP1 (R3 P) = R3 (ACP1 P)" 
+proof -
+have "ACP1 (R3 P) = `($wait \<and> \<not> ok \<and> ($tr \<le> $tr\<acute>)) \<or> (ok' \<and> $wait \<and> II\<^bsub>REL_VAR - {okay\<down>, okay\<down>\<acute>}\<^esub> \<and> ( ok \<and> ($tr =$tr\<acute>) \<Rightarrow> $wait\<acute>)) \<or> (\<not>$wait \<and> P \<and> ( ok \<and> ($tr =$tr\<acute>) \<Rightarrow> $wait\<acute>))`" by (simp add:ACP1_def R3_def SkipREA_def CondR_def, utp_pred_auto_tac)
+also have "... = `($wait \<and> \<not> ok \<and> ($tr \<le> $tr\<acute>)) \<or> (ok' \<and> $wait \<and> $wait\<acute> \<and> II\<^bsub>REL_VAR - {okay\<down>, okay\<down>\<acute>}\<^esub> \<and> ( ok \<and> ($tr =$tr\<acute>) \<Rightarrow> $wait\<acute>)) \<or> (\<not>$wait \<and> P \<and> ( ok \<and> ($tr =$tr\<acute>) \<Rightarrow> $wait\<acute>))`" by (smt AndP_assoc helper1)
+also have "... = `($wait \<and> \<not> ok \<and> ($tr \<le> $tr\<acute>)) \<or> (ok' \<and> $wait \<and> $wait\<acute> \<and> II\<^bsub>REL_VAR - {okay\<down>, okay\<down>\<acute>}\<^esub>) \<or> (\<not>$wait \<and> P \<and> ( ok \<and> ($tr =$tr\<acute>) \<Rightarrow> $wait\<acute>))`" by (utp_pred_auto_tac)
+also have "... = `($wait \<and> \<not> ok \<and> ($tr \<le> $tr\<acute>)) \<or> (ok' \<and> $wait \<and> II\<^bsub>REL_VAR - {okay\<down>, okay\<down>\<acute>}\<^esub>) \<or> (\<not>$wait \<and> P \<and> ( ok \<and> ($tr =$tr\<acute>) \<Rightarrow> $wait\<acute>))`" by (smt helper1)
+also have "... = `R3(P \<and> ( ok \<and> ($tr =$tr\<acute>) \<Rightarrow> $wait\<acute>))`" by(simp add: R3_def CondR_def SkipREA_def, utp_pred_auto_tac)
+finally show ?thesis by(simp add:ACP1_def)
+qed
 
 definition \<delta> :: "'a WF_PREDICATE" where
-"\<delta> = `R3($tr =$tr\<acute> \<and> ($wait)\<acute>)`"
-
-lemma \<delta>_is_R1 : "`R1(\<delta>)` = \<delta>" sorry
-lemma \<delta>_is_R2 : "`R2(\<delta>)` = \<delta>" sorry
-lemma \<delta>_is_R3 : "`R3(\<delta>)` = \<delta>" by (simp add: \<delta>_def R3_idempotent)
-
-lemma \<delta>_closure : "\<delta> is R" by (simp add:is_healthy_def R_def \<delta>_is_R3 \<delta>_is_R2 \<delta>_is_R1)
+"\<delta> = `R3($tr =$tr\<acute> \<and> $wait\<acute>)`"
 
 definition B :: "'a WF_PREDICATE" where
-"B = `($tr =$tr\<acute> \<and> ($wait)\<acute>) \<or> ($tr \<le> $tr\<acute>)`"
+"B = `($tr = $tr\<acute> \<and> $wait\<acute>) \<or> ($tr < $tr\<acute>)`"
 
 definition \<Phi> :: "'a WF_PREDICATE \<Rightarrow> 'a WF_PREDICATE" where
-"\<Phi>(P) = `R1(R3(B \<and> P))`"
+"\<Phi>(P) = `R(B \<and> P)`"
 
 syntax 
   "_upred_Phi" :: "upred \<Rightarrow> upred" ("\<Phi>'(_')")
@@ -38,7 +59,7 @@ translations
   "_upred_Phi P" == "CONST \<Phi> P"
 
 definition doA :: "('m EVENT, 'm) WF_PEXPRESSION \<Rightarrow> 'm WF_PREDICATE" where
-"doA(a) = `\<Phi>(a \<notin> $ref\<acute> \<lhd> $wait \<rhd> ($tr^\<langle>a\<rangle> =$tr\<acute>))`"
+"doA(a) = `\<Phi>(a \<notin> $ref\<acute> \<lhd> $wait\<acute> \<rhd> ($tr^\<langle>a\<rangle> =$tr\<acute>))`"
 
 syntax 
   "_upred_doA" :: "uexpr \<Rightarrow> upred" ("do\<A>'(_')")
@@ -46,37 +67,183 @@ syntax
 translations
   "_upred_doA a" == "CONST doA a"
 
-lemma doA_closure : "(do\<A> a) is R" sorry
-
-lemma L1 : "\<delta> ; P = \<delta>"
-apply (simp add:\<delta>_def R3_def SkipREA_def)
-oops
-
 definition alternative :: "'a WF_PREDICATE \<Rightarrow> 'a WF_PREDICATE \<Rightarrow> 'a WF_PREDICATE" ("_ +\<^bsub>ACP\<^esub> _") where
 "(P +\<^bsub>ACP\<^esub> Q) = `(P \<and> Q)\<lhd> \<delta> \<rhd> (P \<or> Q)`"
 
-lemma alternative_closure :
-  assumes "(P = `P \<and> ($tr \<le> $tr\<acute>)`) \<and> (Q = `Q \<and> ($tr \<le> $tr\<acute>)`)"
-  shows "(P +\<^bsub>ACP\<^esub> Q) is R1"
-apply (simp add: alternative_def is_healthy_def R1_def CondR_def)
-oops
+lemma \<delta>_is_R1 : "`R1(\<delta>)` = `\<delta>`"
+proof -
+have "`R1(\<delta>)`  = `(II\<^bsub>rea\<^esub> \<and> ($tr \<le> $tr\<acute>)) \<lhd> $wait \<rhd> ($tr =$tr\<acute> \<and> $wait\<acute> \<and> ($tr \<le> $tr\<acute>))`" by(simp add:\<delta>_def, utp_pred_auto_tac)
+also have "... = `R1(II\<^bsub>rea\<^esub>) \<lhd> $wait \<rhd> ($tr =$tr\<acute> \<and> $wait\<acute> )`" by(utp_pred_auto_tac)
+finally show ?thesis by (metis SkipREA_is_R1 R3_def \<delta>_def)
+qed
 
+lemma \<delta>_is_R2 : "`R2(\<delta>)` = `\<delta>`" 
+proof -
+have "`R2(\<delta>)`= `R3(R2($tr = $tr\<acute>) \<and> $wait\<acute>)`"by(simp add:\<delta>_def R2_R3_commute, simp add:R2_def R1_def R2s_def usubst typing closure defined, utp_pred_auto_tac)
+thus ?thesis by (simp add:R2_def tr_conserved_is_R2 tr_conserved_is_R1 \<delta>_def)
+qed
 
-lemma L2 : "P +\<^bsub>ACP\<^esub> P = P"
-oops
+lemma \<delta>_is_R3 : "`R3(\<delta>)` = `\<delta>`" by (simp add: \<delta>_def R3_idempotent)
 
-lemma L3 : "P +\<^bsub>ACP\<^esub> Q = Q +\<^bsub>ACP\<^esub> P"
-oops
+lemma \<delta>_closure : "\<delta> is R" by (simp add: is_healthy_def R_def \<delta>_is_R3 \<delta>_is_R2 \<delta>_is_R1)
 
-lemma L4 : "(P +\<^bsub>ACP\<^esub> Q)+\<^bsub>ACP\<^esub> S = P +\<^bsub>ACP\<^esub> (Q +\<^bsub>ACP\<^esub> S)"
-oops
+lemma \<delta>_is_ACP1 : "\<delta> is ACP1" by(simp add:is_healthy_def \<delta>_def ACP1_R3_commute, simp add:ACP1_def, utp_pred_auto_tac)
 
-lemma L5 : "\<delta> +\<^bsub>ACP\<^esub> Q = Q"
-oops
+lemma \<delta>_form : "\<delta> = `(\<not> ok \<and> $wait \<and> ($tr \<le> $tr\<acute>)) \<or> $wait\<acute> \<and>  ((ok' \<and> $wait \<and> II\<^bsub>REL_VAR - {okay\<down>, okay\<down>\<acute>}\<^esub>) \<or> (\<not>$wait \<and> ($tr = $tr\<acute>)))`"
+proof - 
+have "\<delta> = `(\<not> ok \<and> $wait \<and> ($tr \<le> $tr\<acute>)) \<or> ((ok' \<and> $wait \<and> II\<^bsub>REL_VAR - {okay\<down>, okay\<down>\<acute>}\<^esub>) \<or> (\<not>$wait \<and> $wait\<acute> \<and>  ($tr = $tr\<acute>)))`" by(simp add:\<delta>_def R3_def SkipREA_def CondR_def,utp_pred_auto_tac)
+also have "... = `(\<not> ok \<and> $wait \<and> ($tr \<le> $tr\<acute>)) \<or> $wait\<acute> \<and> ((ok' \<and> $wait \<and> II\<^bsub>REL_VAR - {okay\<down>, okay\<down>\<acute>}\<^esub>) \<or> (\<not>$wait \<and> ($tr = $tr\<acute>)))`"by(simp add:helper1, utp_pred_auto_tac)
+finally show ?thesis ..
+qed 
+
+lemma doA_is_R1 : "`R1(do\<A>(a))` = `do\<A>(a)`"by(simp add:doA_def \<Phi>_def R_def R1_idempotent)
+lemma doA_is_R2 : "`R2(do\<A>(a))` = `do\<A>(a)`"by(simp add:doA_def \<Phi>_def R_def R1_R2_commute R2_idempotent)
+lemma doA_is_R3 : "`R3(do\<A>(a))` = `do\<A>(a)`"by(simp add:doA_def \<Phi>_def R_def R2_R3_commute R1_R3_commute R3_idempotent)
+
+lemma doA_closure : "`do\<A>(a)` is R" by(simp add:is_healthy_def R_def doA_is_R3 doA_is_R2 doA_is_R1)
+
+lemma doA_is_ACP1 :"`do\<A>(a)` is ACP1" 
+proof -
+have "`ACP1(B \<and>( a \<notin> $ref\<acute> \<lhd> $wait\<acute> \<rhd> ($tr^\<langle>a\<rangle> =$tr\<acute>)))` = `(B \<and>( a \<notin> $ref\<acute> \<lhd> $wait\<acute> \<rhd> ($tr^\<langle>a\<rangle> =$tr\<acute>)))`" by(simp add:ACP1_def CondR_def, utp_pred_auto_tac)
+moreover have "`ACP1(do\<A>(a))` = `R(ACP1(B \<and>( a \<notin> $ref\<acute> \<lhd> $wait\<acute> \<rhd> ($tr^\<langle>a\<rangle> =$tr\<acute>))))`" by(simp add:doA_def \<Phi>_def R_def ACP1_R1_commute ACP1_R2_commute ACP1_R3_commute)
+ultimately show ?thesis by(simp add:is_healthy_def doA_def \<Phi>_def)
+qed
+
+lemma B_form : "B = `R1($wait\<acute> \<or> ($tr < $tr\<acute>))`"sorry
+lemma a_unrest : "`a[\<langle>\<rangle>/tr][($tr\<acute> - $tr)/tr\<acute>]` = `a`"sorry
+lemma aider : "`(B \<and> ((a \<notin> $ref\<acute>) \<lhd> $wait\<acute> \<rhd> ($tr ^ \<langle>a\<rangle> = $tr\<acute>)))` = `((a \<notin> $ref\<acute>) \<and> ($tr \<le> $tr\<acute>)) \<lhd> $wait\<acute> \<rhd> (($tr ^ \<langle>a\<rangle> = $tr\<acute>) \<and> ($tr < $tr\<acute>))`"by(simp add:B_form, utp_pred_auto_tac)
+lemma aider2 : "`R2s(((a \<notin> $ref\<acute>) \<and> ($tr \<le> $tr\<acute>)) \<lhd> $wait\<acute> \<rhd> (($tr ^ \<langle>a\<rangle> = $tr\<acute>) \<and> ($tr < $tr\<acute>)))` = `(a \<notin> $ref\<acute>) \<lhd> $wait\<acute> \<rhd> ($tr ^ \<langle>a\<rangle> = $tr\<acute>)`"
+proof-
+have "`R2s(((a \<notin> $ref\<acute>) \<and> ($tr \<le> $tr\<acute>)) \<lhd> $wait\<acute> \<rhd> (($tr ^ \<langle>a\<rangle> = $tr\<acute>) \<and> ($tr < $tr\<acute>)))` = `((a[\<langle>\<rangle>/tr][($tr\<acute> - $tr)/tr\<acute>] \<notin> $ref\<acute>) \<and> (\<langle>\<rangle> \<le> $tr\<acute> - $tr)) \<lhd> $wait\<acute> \<rhd> (\<langle>\<rangle> ^ \<langle>a[\<langle>\<rangle>/tr][($tr\<acute> - $tr)/tr\<acute>]\<rangle> = ($tr\<acute> - $tr) \<and> (\<langle>\<rangle> < $tr\<acute> - $tr))`" by(simp add:R2s_def usubst typing closure defined)
+also have "... = `((a[\<langle>\<rangle>/tr][($tr\<acute> - $tr)/tr\<acute>] \<notin> $ref\<acute>)) \<lhd> $wait\<acute> \<rhd> (\<langle>a[\<langle>\<rangle>/tr][($tr\<acute> - $tr)/tr\<acute>]\<rangle> = ($tr\<acute> - $tr) \<and> (\<langle>\<rangle> < ($tr\<acute> - $tr)))`" by(utp_pred_auto_tac)
+finally show ?thesis sorry qed
+
+lemma doA_form : "`do\<A>(a)` = `R3(((a \<notin> $ref\<acute>) \<and> ($tr \<le> $tr\<acute>)) \<lhd> $wait\<acute> \<rhd> ($tr ^ \<langle>a\<rangle> = $tr\<acute>))`"
+proof -
+have "`do\<A>(a)` = `R(B \<and> ((a \<notin> $ref\<acute>) \<lhd> $wait\<acute> \<rhd> ($tr ^ \<langle>a\<rangle> = $tr\<acute>)))`" by(simp add: doA_def \<Phi>_def)
+also have "... = `R(((a \<notin> $ref\<acute>) \<and> ($tr \<le> $tr\<acute>)) \<lhd> $wait\<acute> \<rhd> (($tr ^ \<langle>a\<rangle> = $tr\<acute>) \<and> ($tr < $tr\<acute>)))`" by(metis aider)
+also have "... = `R3(R1(R2s(((a \<notin> $ref\<acute>) \<and> ($tr \<le> $tr\<acute>)) \<lhd> $wait\<acute> \<rhd> (($tr ^ \<langle>a\<rangle> = $tr\<acute>) \<and> ($tr < $tr\<acute>)))))`" by(simp add:R_def R2_R3_commute R1_R3_commute, simp add:R2_def R1_idempotent)
+also have "... = `R3(R1((a \<notin> $ref\<acute>) \<lhd> $wait\<acute> \<rhd> ($tr ^ \<langle>a\<rangle> = $tr\<acute>)))`" by(metis aider2)
+also have "... = `R3(((a \<notin> $ref\<acute>) \<and> ($tr \<le> $tr\<acute>)) \<lhd> $wait\<acute> \<rhd> (($tr ^ \<langle>a\<rangle> = $tr\<acute>) \<and> ($tr \<le> $tr\<acute>)))`" by(utp_pred_auto_tac)
+finally show ?thesis sorry qed
+
+lemma alternative_is_R1 :
+  assumes "P is R1 \<and> Q is R1"
+  shows "P +\<^bsub>ACP\<^esub> Q is R1"
+using assms
+by (simp add:alternative_def is_healthy_def R1_def, utp_pred_auto_tac)
+
+lemma alternative_is_R2 :
+  assumes "P is R2 \<and> Q is R2"
+  shows "(P +\<^bsub>ACP\<^esub> Q) is R2"
+using assms
+proof -
+have "R2 (P +\<^bsub>ACP\<^esub> Q) =  `R2(P \<and> Q) \<lhd> R2(\<delta>) \<rhd> R2(P \<or> Q)`" by (simp add:alternative_def R2_distributes_through_conditional CondR_def R2_def R1_def, utp_pred_auto_tac)
+also have "... = `(R2(P) \<and> R2(Q)) \<lhd> \<delta> \<rhd> (R2(P) \<or> R2(Q))`" by (simp add: \<delta>_is_R2, simp add: R2_def R1_def R2s_def usubst, utp_pred_auto_tac)
+moreover from assms have "... = `(P \<and> Q) \<lhd> \<delta> \<rhd> (P \<or> Q)`" by(simp add:is_healthy_def)
+ultimately show ?thesis by (simp add:is_healthy_def alternative_def)
+qed
+
+lemma alternative_is_R3 : 
+  assumes "P is R3 \<and> Q is R3"
+  shows "(P +\<^bsub>ACP\<^esub> Q) is R3"
+using assms
+proof -
+from assms have "`P \<and> Q` is R3" by(simp add:is_healthy_def R3_def, utp_pred_auto_tac)
+moreover from assms have "`P \<or> Q` is R3" by(simp add:is_healthy_def R3_distributes_through_disjunction)
+ultimately show ?thesis by(simp add:is_healthy_def alternative_def R3_distributes_through_conditional \<delta>_is_R3) 
+qed
+
+lemma alternative_closure : 
+  assumes "P is R \<and> Q is R"
+  shows "P +\<^bsub>ACP\<^esub> Q is R"
+using assms
+proof - 
+from assms have "P is R3 \<and> Q is R3"
+proof -
+  from assms have "P is R3" proof-
+    from assms have "`R3(P)` = `R3(R(P))`" pr by (simp add:is_healthy_def)
+    also have "... = `R(P)`" by (simp add:R_def R2_R3_commute R1_R3_commute R3_idempotent)
+    also from assms have "... = `P`" by (simp add:is_healthy_def)
+    finally show ?thesis by (simp add:is_healthy_def)
+  qed
+  moreover from assms have "Q is R3" 
+  proof -
+    from assms have "`R3(Q)` = `R3(R(Q))`" by (simp add:is_healthy_def)
+    also have "... = `R(Q)`" by (simp add:R_def R2_R3_commute R1_R3_commute R3_idempotent)
+    also from assms have "... = `Q`" by (simp add:is_healthy_def)
+    finally show ?thesis by (simp add:is_healthy_def)
+  qed
+  ultimately show ?thesis ..
+qed
+hence "P +\<^bsub>ACP\<^esub> Q is R3" by (simp add:alternative_is_R3)
+moreover from assms have "P is R2 \<and> Q is R2" 
+proof -
+  from assms have "P is R2" proof-
+    from assms have "`R2(P)` = `R2(R(P))`" pr by (simp add:is_healthy_def)
+    also have "... = `R(P)`" by (simp add:R_def R1_R2_commute R2_idempotent)
+    also from assms have "... = `P`" by (simp add:is_healthy_def)
+    finally show ?thesis by (simp add:is_healthy_def)
+  qed
+  moreover from assms have "Q is R2" 
+  proof -
+    from assms have "`R2(Q)` = `R2(R(Q))`" by (simp add:is_healthy_def)
+    also have "... = `R(Q)`" by (simp add:R_def R1_R2_commute R2_idempotent)
+    also from assms have "... = `Q`" by (simp add:is_healthy_def)
+    finally show ?thesis by (simp add:is_healthy_def)
+  qed
+  ultimately show ?thesis ..
+qed
+hence "P +\<^bsub>ACP\<^esub> Q is R2" by (simp add:alternative_is_R2)
+moreover from assms have "P is R1 \<and> Q is R1" 
+proof -
+  from assms have "P is R1" proof-
+    from assms have "`R1(P)` = `R1(R(P))`" pr by (simp add:is_healthy_def)
+    also have "... = `R(P)`" by (simp add:R_def R1_idempotent)
+    also from assms have "... = `P`" by (simp add:is_healthy_def)
+    finally show ?thesis by (simp add:is_healthy_def)
+  qed
+  moreover from assms have "Q is R1" 
+  proof -
+    from assms have "`R1(Q)` = `R1(R(Q))`" by (simp add:is_healthy_def)
+    also have "... = `R(Q)`" by (simp add:R_def R1_idempotent)
+    also from assms have "... = `Q`" by (simp add:is_healthy_def)
+    finally show ?thesis by (simp add:is_healthy_def)
+  qed
+  ultimately show ?thesis ..
+qed
+hence "P +\<^bsub>ACP\<^esub> Q is R1" by (simp add:alternative_is_R1)
+ultimately show ?thesis by (simp add: is_healthy_def R_def)
+qed
+
+lemma alternative_is_ACP1 :
+  assumes "P is ACP1 \<and> Q is ACP1"
+  shows "(P +\<^bsub>ACP\<^esub> Q) is ACP1"
+using assms
+by(simp add:is_healthy_def ACP1_def alternative_def, utp_pred_auto_tac)
+
+lemma L1 :
+  assumes "P is R3"
+  shows "\<delta> ; P = \<delta>"
+using assms
+proof -
+from assms have "\<delta> ; P = `((\<not> ok \<and> $wait \<and> ($tr \<le> $tr\<acute>)); P) \<or> ($wait\<acute> \<and> ((ok' \<and> $wait \<and> II\<^bsub>REL_VAR - {okay\<down>, okay\<down>\<acute>}\<^esub>) \<or> \<not>$wait \<and> ($tr = $tr\<acute>))) ; R3(P)`"by(simp add:is_healthy_def \<delta>_form SemiR_OrP_distr)
+also have "... = `(\<not> ok \<and> $wait \<and> ($tr \<le> $tr\<acute>)) \<or> ($wait\<acute> \<and>  ((ok' \<and> $wait \<and> II\<^bsub>REL_VAR - {okay\<down>, okay\<down>\<acute>}\<^esub>) \<or> \<not>$wait \<and> ($tr = $tr\<acute>))) ; R3(P)`" by(simp add:helper3)
+also have "... = `(\<not> ok \<and> $wait \<and> ($tr \<le> $tr\<acute>)) \<or> ($wait\<acute> \<and>  ((ok' \<and> $wait \<and> II\<^bsub>REL_VAR - {okay\<down>, okay\<down>\<acute>}\<^esub>) \<or> \<not>$wait \<and> ($tr = $tr\<acute>)))`" by(metis helper2)
+also have "... = `(\<not> ok \<and> $wait \<and> ($tr \<le> $tr\<acute>)) \<or> (ok' \<and> $wait \<and> II\<^bsub>REL_VAR - {okay\<down>, okay\<down>\<acute>}\<^esub>) \<or> \<not>$wait \<and> $wait\<acute> \<and> ($tr = $tr\<acute>)`" by(simp add:helper1, utp_pred_auto_tac)
+also have "... = \<delta>" by(simp add:\<delta>_def R3_def CondR_def SkipREA_def, utp_pred_auto_tac)
+finally show ?thesis ..
+qed
+
+lemma L2 : "P +\<^bsub>ACP\<^esub> P= P" by(simp add: alternative_def, utp_pred_auto_tac)
+
+lemma L3 : "P +\<^bsub>ACP\<^esub> Q = Q +\<^bsub>ACP\<^esub> P" by(simp add:alternative_def, utp_pred_auto_tac)
+
+lemma L4 : "(P +\<^bsub>ACP\<^esub> Q)+\<^bsub>ACP\<^esub> S = P +\<^bsub>ACP\<^esub> (Q +\<^bsub>ACP\<^esub> S)" by(simp add:alternative_def, utp_pred_auto_tac)
+
+lemma L5 : "\<delta> +\<^bsub>ACP\<^esub> Q = Q" by(simp add:alternative_def, utp_pred_auto_tac)
 
 lemma L6 : "(P +\<^bsub>ACP\<^esub> Q) ; S = (P;S) +\<^bsub>ACP\<^esub> (Q;S)"
-oops
-
-
-
+apply(simp add:alternative_def CondR_def SemiR_OrP_distr)
+sorry
 end
