theories/theories/utp_csp.thy
@@ -8,8 +8,6 @@ header {* CSP Processes *}
 
 theory utp_csp
 imports 
-  utp_designs
-  utp_theory
   utp_reactive
   utp_acp
 begin
@@ -57,47 +55,51 @@ declare doA_def [eval, evalr, evalrr, evalrx]
 declare \<Phi>_def [eval, evalr, evalrr, evalrx]
 declare B_def [eval, evalr, evalrr, evalrx]
 
-lemma CSP1_idempotent:
-  assumes "P is CSP1"
-  shows "CSP1 P = P" 
-using assms
-by (utp_rel_tac)
+lemma J_rea_is_CSP2 : "`J\<^bsub>rea\<^esub> ; J\<^bsub>rea\<^esub>` = `J\<^bsub>rea\<^esub>`"sorry
+lemma CSP1_false_is_CSP2 : "`(\<not> ok \<and> ($tr \<le> $tr\<acute>)) ; J\<^bsub>rea\<^esub>` = `(\<not> ok \<and> ($tr \<le> $tr\<acute>))`" sorry
+lemma \<delta>_and_SKIP_is_false : "`((ok\<acute> \<and> \<delta>) \<and> (\<not> ok \<and> ($tr \<le> $tr\<acute>)) \<and> SKIP) ; J\<^bsub>rea\<^esub> \<or> Q` = `Q`" sorry
+lemma aid : "`((\<not> ok \<and> ($tr \<le> $tr\<acute>)) \<and> (\<not> ok \<and> ($tr \<le> $tr\<acute>)) \<and> SKIP) ; J\<^bsub>rea\<^esub>` =`(\<not> ok \<and> ($tr \<le> $tr\<acute>))`" oops
+lemma CSP2_form: "`CSP2(P)` = `P\<^sup>f \<or> ok'\<and> P\<^sup>t`"sorry
+lemma SkipREA_is_CSP2 : "`CSP2(II\<^bsub>rea\<^esub>)` = `II\<^bsub>rea\<^esub>`"sorry
+lemma R3_form : "`R3(P)` = `II\<^bsub>rea\<^esub> \<lhd> $wait \<rhd> (P\<^sub>f)`"sorry
 
-lemma CSP2_idempotent:
-  assumes "P is CSP2"
-  shows "CSP2 P = P" 
-using assms
-by (utp_rel_tac)
+lemma CSP1_idempotent: "`CSP1(CSP1(P))` = `CSP1(P)`" by(utp_pred_auto_tac)
+lemma CSP2_idempotent: "`CSP2(CSP2(P))` = `CSP2(P)`" by(simp add: CSP2_def seq_comp_assoc J_rea_is_CSP2)
 
 lemma CSP1_monotonic: "[P\<Rightarrow>Q] \<Longrightarrow> [CSP1(P) \<Rightarrow> CSP1(Q)]"by (utp_pred_tac)
-lemma CSP2_monotonic: "[P\<Rightarrow>Q] \<Longrightarrow> [CSP2(P) \<Rightarrow> CSP2(Q)]"sorry
+lemma CSP2_monotonic: "[P\<Rightarrow>Q] \<Longrightarrow> [CSP2(P) \<Rightarrow> CSP2(Q)]"by(simp add:CSP2_form, utp_pred_auto_tac)
 
-lemma CSP1_false_is_CSP2 : "`(\<not> ok \<and> ($tr \<le> $tr\<acute>)) ; J\<^bsub>rea\<^esub>` = `(\<not> ok \<and> ($tr \<le> $tr\<acute>))`" sorry
-
-lemma CSP1_CSP2_commute: "CSP1 (CSP2 P) = CSP2 (CSP1 P)"
+lemma CSP1_CSP2_commute: "CSP1 (CSP2 P) = CSP2 (CSP1 P)"by(simp add:CSP2_form CSP1_def usubst typing defined closure, utp_pred_auto_tac)
+lemma CSP1_R1_commute: "CSP1 (R1 P) = R1 (CSP1 (P))"by utp_pred_auto_tac
+lemma CSP1_R2_commute: "CSP1 (R2 P) = R2 (CSP1 (P))"by(simp add:CSP1_def R2_def R2s_def usubst typing defined closure, utp_pred_auto_tac)
+lemma CSP1_R3_commute: "CSP1 (R3 P) = R3 (CSP1 (P))"by utp_pred_auto_tac
+lemma CSP2_R1_commute: "CSP2 (R1 P) = R1 (CSP2 (P))"by (simp add:CSP2_form, utp_pred_auto_tac)
+lemma CSP2_R2_commute: "CSP2 (R2 P) = R2 (CSP2 (P))"sorry
+lemma CSP2_R3_commute: "CSP2 (R3 P) = R3 (CSP2 (P))" 
 proof -
-  have "CSP2 (CSP1 P) = `(P \<or> \<not> ok \<and> ($tr \<le> $tr\<acute>)) ; J\<^bsub>rea\<^esub>`" by (utp_rel_tac)
-  also have "... = `(P ; J\<^bsub>rea\<^esub>) \<or> (\<not> ok \<and> ($tr \<le> $tr\<acute>)) ; J\<^bsub>rea\<^esub>`" sorry
-  ultimately show ?thesis by (simp add: CSP1_false_is_CSP2, utp_rel_tac)
+have "CSP2 (R3 P) = `($wait \<and> CSP2(II\<^bsub>rea\<^esub>)) \<or> (\<not> $wait \<and> CSP2(P))`" 
+  apply(simp add:CSP2_form R3_def CondR_def usubst typing defined closure)
+  apply utp_pred_auto_tac
+done
+thus ?thesis by (simp add:SkipREA_is_CSP2 CondR_def R3_def)
 qed
 
-lemma R2_distributes_through_disjunction: "`R2(A \<or> C)` = `R2(A) \<or> R2(C)`" sorry
-lemma R1_not_ok : "`(\<not> ok \<and> ($tr \<le> $tr\<acute>))` = `R1(\<not> ok)`"sorry
-lemma R2_R1_commute :"`R2(R1(P))` = `R1(R2(P))`"sorry
-lemma not_ok_is_R2 : "`R2(\<not> ok)` = `\<not> ok`"sorry
+lemma commuting_substitutions : "`R2s(P)[false/wait]` = `R2s(P [false/wait])`" apply(simp add:R2s_def)  sorry
 
-lemma CSP1_R1_commute: "CSP1 (R1 P) = R1 (CSP1 (P))"by (simp add: CSP1_def R1_def, utp_pred_auto_tac)
-lemma CSP1_R2_commute: "CSP1 (R2 P) = R2 (CSP1 (P))"by (simp add: CSP1_def R2_distributes_through_disjunction R1_not_ok R2_R1_commute not_ok_is_R2)
-lemma CSP1_R3_commute: "CSP1 (R3 P) = R3 (CSP1 (P))"by (simp add: CSP1_def R3_def CondR_def SkipREA_def, utp_pred_auto_tac)
-lemma CSP2_R1_commute: "CSP2 (R1 P) = R1 (CSP2 (P))"sorry
-lemma CSP2_R2_commute: "CSP2 (R2 P) = R2 (CSP2 (P))"sorry
-lemma CSP2_R3_commute: "CSP2 (R3 P) = R3 (CSP2 (P))"sorry
-lemma CSP_Closure : "P is CSP \<longleftrightarrow> P = `R(\<not> P\<^sup>f\<^sub>f \<turnstile> P\<^sup>t\<^sub>f)`"sorry 
-
-lemma CSP_Assignment : "`R(x:= e)` is (CSP1 \<circ> CSP2)" sorry
-
-definition assignment :: "('a::type,'m::REACTIVE_SORT) PVAR \<Rightarrow> ('a,'m) WF_PEXPRESSION \<Rightarrow> 'm WF_PREDICATE" ("_:=\<^bsub>CSP\<^esub>_")where
-"x:=\<^bsub>CSP\<^esub>e =`R(x:=e)`"
+lemma CSP_Closure : "P is CSP \<longleftrightarrow> `R(\<not> P\<^sup>f\<^sub>f \<turnstile> P\<^sup>t\<^sub>f)` = P"
+proof -
+have "`R(\<not> P\<^sup>f\<^sub>f \<turnstile> P\<^sup>t\<^sub>f)` = `R1(R3( \<not>ok \<or> R2s(P\<^sup>f\<^sub>f) \<or> R2s(ok'\<and>  P\<^sup>t\<^sub>f)))`" by(simp add:R_def R2_def R1_idempotent R2s_R3_commute DesignD_form R2s_distributes_through_disjunction not_ok_is_R2s)
+also have "... = `R1(($wait \<and> II\<^bsub>rea\<^esub>) \<or> (\<not>$wait \<and> \<not>ok) \<or> (\<not>$wait \<and> R2s(P\<^sup>f\<^sub>f)) \<or> (\<not>$wait\<and> ok'\<and> R2s(P\<^sup>t\<^sub>f)))`" by(simp add:R3_def CondR_def R2s_distributes_through_conjunction ok_dash_is_R2s, utp_pred_auto_tac)
+also have "... = `($wait \<and> \<not>ok \<and> ($tr \<le> $tr\<acute>)) \<or> ($wait \<and> ok' \<and> ($tr \<le> $tr\<acute>) \<and> II\<^bsub>REL_VAR - {okay\<down>, okay\<down>\<acute>}\<^esub>) \<or> (\<not>$wait \<and> ($tr \<le> $tr\<acute>) \<and> \<not>ok) \<or> (\<not>$wait \<and> ($tr \<le> $tr\<acute>) \<and> R2s(P\<^sup>f\<^sub>f)) \<or> (\<not>$wait\<and> ok'\<and> ($tr \<le> $tr\<acute>) \<and> R2s(P\<^sup>t\<^sub>f))`" by utp_pred_auto_tac
+also have "... = `(\<not>ok \<and> ($tr \<le> $tr\<acute>)) \<or> ($wait \<and> \<not>ok \<and> ($tr \<le> $tr\<acute>)) \<or> ($wait \<and> ok' \<and> ($tr \<le> $tr\<acute>) \<and> II\<^bsub>REL_VAR - {okay\<down>, okay\<down>\<acute>}\<^esub>) \<or> (\<not>$wait \<and> ($tr \<le> $tr\<acute>) \<and> R2(P\<^sup>f\<^sub>f)) \<or> (\<not>$wait\<and> ok'\<and> ($tr \<le> $tr\<acute>) \<and> R2s(P\<^sup>t\<^sub>f))`" by utp_pred_auto_tac
+also have "... = `CSP1(R1(($wait \<and> ( \<not>ok  \<or> (ok'  \<and> II\<^bsub>REL_VAR - {okay\<down>, okay\<down>\<acute>}\<^esub>))) \<or> (\<not>$wait \<and> (R2s(P\<^sup>f\<^sub>f) \<or> (ok'\<and> R2s(P\<^sup>t\<^sub>f))))))`" by utp_pred_auto_tac
+also have "... = `CSP1(R1(($wait \<and> ( \<not>ok  \<or> (ok'  \<and> II\<^bsub>REL_VAR - {okay\<down>, okay\<down>\<acute>}\<^esub>))) \<or> (\<not>$wait \<and> (R2s(P\<^sup>f) \<or> (ok'\<and> R2s(P\<^sup>t)))\<^sub>f)))`" by(simp add:usubst typing closure defined, simp add:commuting_substitutions)
+also have "... = `CSP1(R1(R3(R2s(P\<^sup>f) \<or> ( ok'\<and> R2s(P\<^sup>t)))))`" by(simp add:R3_form CondR_def SkipREA_def, utp_pred_auto_tac)
+also have "... = `CSP1(R1(R3(R2s(P\<^sup>f \<or> ( ok'\<and> P\<^sup>t)))))`" by (simp add:R2s_distributes_through_disjunction R2s_distributes_through_conjunction ok_dash_is_R2s)
+also have "... = `CSP1(R1(R2(R3(CSP2(P)))))`" by(simp add:R2_def R1_idempotent R2s_R3_commute CSP2_form)
+also have "... = `CSP(P)`" by (simp add:CSP_def R_def CSP2_R1_commute CSP2_R2_commute CSP2_R3_commute)
+finally show ?thesis by(simp add:is_healthy_def)
+qed
 
 definition deadlock :: "'a WF_PREDICATE" ("STOP") where
 "STOP = `CSP1( ok' \<and> \<delta>)`"
@@ -123,30 +125,6 @@ translations
   "_upred_skip" == "CONST SkipCSP"
   "_upred_chaos" == "CONST ChaosCSP"
 
-declare deadlock_def [eval, evalr, evalrr, evalrx]
-declare prefix_def [eval, evalr, evalrr, evalrx]
-declare SkipCSP_def [eval, evalr, evalrr, evalrx]
-declare ChaosCSP_def [eval, evalr, evalrr, evalrx]
-
-lemma Stop_form : "`STOP`= `(\<not> ok \<and> ($tr \<le> $tr\<acute>)) \<or> ($wait \<and> ok' \<and> II\<^bsub>REL_VAR - OKAY\<^esub>) \<or> (\<not> $wait \<and> ok' \<and> \<delta>)`" by (utp_pred_auto_tac)
-lemma Prefix_form : "`@a`= `(\<not> ok \<and> ($tr \<le> $tr\<acute>)) \<or> ($wait \<and> ok' \<and> II\<^bsub>REL_VAR - OKAY\<^esub> \<and> ($tr \<le> $tr\<acute>))\<or> (\<not> $wait \<and> ok' \<and> do\<A>(a))`"by (utp_pred_auto_tac)
-lemma Skip_form : "`SKIP`= `(\<not> ok \<and> ($tr \<le> $tr\<acute>)) \<or> ($wait \<and> ok' \<and> II\<^bsub>REL_VAR - OKAY\<^esub>) \<or> (\<not> $wait \<and> ok' \<and> (\<exists> ref .II\<^bsub>rea\<^esub>))`"by (utp_pred_auto_tac)
-lemma Chaos_form : "`CHAOS`= `(\<not> ok \<and> ($tr \<le> $tr\<acute>)) \<or> ($wait \<and> ok' \<and> II\<^bsub>REL_VAR - OKAY\<^esub> \<and> ($tr \<le> $tr\<acute>)) \<or> (\<not> $wait \<and> ($tr \<le> $tr\<acute>))`"by (utp_pred_auto_tac)
-
-lemma CSP1_false_zero_seq_comp :
-  assumes "P is CSP1"
-  shows "`(\<not> ok \<and> ($tr \<le> $tr\<acute>)) ; P` = `(\<not> ok \<and> ($tr \<le> $tr\<acute>))`"
-sorry
-
-lemma wait_is_R2 : "`$wait[($tr\<acute> - $tr)/tr\<acute>][\<langle>\<rangle>/tr]` = `$wait`" sorry
-lemma not_wait_is_R2 : "`(\<not> $wait)[($tr\<acute> - $tr)/tr\<acute>][\<langle>\<rangle>/tr]` = `\<not> $wait`" sorry
-lemma wait_then_P_equals_wait : "`(($wait \<and> II\<^bsub>rea\<^esub>) \<and> ($tr \<le> $tr\<acute>)) ; P` = `(($wait \<and> II\<^bsub>rea\<^esub>) \<and> ($tr \<le> $tr\<acute>))`" sorry
-
-lemma L1 : "`CHAOS ; P` = `CHAOS`"
-sorry
-
-lemma L2 : "`STOP ; P` = `STOP`"
-sorry
 
 definition prefixed :: "('a EVENT, 'a) WF_PEXPRESSION \<Rightarrow> 'a WF_PREDICATE \<Rightarrow> 'a WF_PREDICATE" ("_\<rightarrow>_") where
 "a\<rightarrow>P = `@a ; P`"
@@ -154,28 +132,106 @@ definition prefixed :: "('a EVENT, 'a) WF_PEXPRESSION \<Rightarrow> 'a WF_PREDIC
 definition extchoice :: "'a WF_PREDICATE \<Rightarrow> 'a WF_PREDICATE \<Rightarrow> 'a WF_PREDICATE" ("_\<box>_") where
 "P\<box>Q = `CSP2((P \<and> Q)\<lhd> STOP \<rhd>(P \<or> Q))`"
 
+definition N :: "('a EVENT UFSET, 'a) WF_PEXPRESSION \<Rightarrow> ('a VAR set * 'a WF_PREDICATE)" where
+"N A = ({okay\<down>\<acute>, wait\<down>\<acute>, ref\<down>\<acute>, tr\<down>\<acute>}, `(($okay\<acute> = $okay\<^bsub>0\<^esub>\<acute> \<and> $okay\<^bsub>1\<^esub>\<acute>) \<and> ($wait\<acute> = $wait\<^bsub>0\<^esub>\<acute> \<or> $wait\<^bsub>1\<^esub>\<acute>) \<and> ($ref\<acute> = $ref\<^bsub>0\<^esub>\<acute> \<union> $ref\<^bsub>1\<^esub>\<acute>) \<and> (($tr\<acute> - $tr)\<in>($tr\<^bsub>0\<^esub> - $tr)\<parallel>\<^bsub>A\<^esub>($tr\<^bsub>1\<^esub>-$tr))); SKIP`)"
+
+definition ParallelCSP :: "'a WF_PREDICATE \<Rightarrow> ('a EVENT UFSET, 'a) WF_PEXPRESSION \<Rightarrow> 'a WF_PREDICATE \<Rightarrow> 'a WF_PREDICATE" (infix "\<parallel>\<^bsub>CSP'(_')\<^esub>" 100) where
+"P \<parallel>\<^bsub>CSP(A)\<^esub> Q = P \<parallel>\<^bsub>N A\<^esub> Q"
+
 syntax
   "_upred_prefixed" :: "pexpr \<Rightarrow> upred \<Rightarrow> upred" ("_\<rightarrow>_")
   "_upred_extchoice" :: "upred \<Rightarrow> upred \<Rightarrow> upred" ("_\<box>_")
+  "_upred_parallel" :: "upred \<Rightarrow> pexpr \<Rightarrow> upred \<Rightarrow> upred" ("_\<parallel>\<^bsub>_\<^esub>_")
   
 translations
   "_upred_prefixed a P" == "CONST prefixed a P"
   "_upred_extchoice P Q" == "CONST extchoice P Q"
+  "_upred_parallel P A Q" == "CONST ParallelCSP P A Q"
+
+definition InterleaveCSP :: "'a WF_PREDICATE \<Rightarrow> 'a WF_PREDICATE \<Rightarrow> 'a WF_PREDICATE" (infix "|||\<^bsub>CSP\<^esub>" 100) where
+"P |||\<^bsub>CSP\<^esub> Q = `P \<parallel>\<^bsub> {} \<^esub> Q`"
+
+syntax
+  "_upred_interleave" :: "upred \<Rightarrow> upred \<Rightarrow> upred" ("_|||_")
+ 
+translations
+  "_upred_interleave P Q" == "CONST InterleaveCSP P Q"
+
+declare deadlock_def [eval, evalr, evalrr, evalrx]
+declare prefix_def [eval, evalr, evalrr, evalrx]
+declare SkipCSP_def [eval, evalr, evalrr, evalrx]
+declare ChaosCSP_def [eval, evalr, evalrr, evalrx]
+declare prefixed_def [eval, evalr, evalrr, evalrx]
+declare extchoice_def [eval, evalr, evalrr, evalrx]
+declare N_def [eval, evalr, evalrr, evalrx]
+declare ParallelCSP_def [eval, evalr, evalrr, evalrx]
+declare InterleaveCSP_def [eval, evalr, evalrr, evalrx]
+
+lemma Stop_form : "`STOP`= `(\<not> ok \<and> ($tr \<le> $tr\<acute>)) \<or> ($wait \<and> ok' \<and> II\<^bsub>REL_VAR - OKAY\<^esub>) \<or> (\<not> $wait \<and> ok' \<and> \<delta>)`" by (utp_pred_auto_tac)
+lemma Prefix_form : "`@a`= `(\<not> ok \<and> ($tr \<le> $tr\<acute>)) \<or> ($wait \<and> ok' \<and> II\<^bsub>REL_VAR - OKAY\<^esub>) \<or> (\<not> $wait \<and> ok' \<and> $wait\<acute> \<and> (a \<notin> $ref\<acute>) \<and> ($tr \<le> $tr\<acute>)) \<or> (\<not> $wait \<and> ok' \<and> \<not> $wait\<acute> \<and> ($tr ^ \<langle>a\<rangle> = $tr\<acute>))`" 
+proof-
+have "`@a`=  `(\<not> ok \<and> ($tr \<le> $tr\<acute>)) \<or> ($wait \<and> ok' \<and> II\<^bsub>REL_VAR - OKAY\<^esub>) \<or> (\<not> $wait \<and> ok' \<and> (((a \<notin> $ref\<acute>) \<and> ($tr \<le> $tr\<acute>)) \<lhd> $wait\<acute> \<rhd> ($tr ^ \<langle>a\<rangle> = $tr\<acute>)))`" by (simp add:prefix_def CSP1_def doA_form R3_def, utp_pred_auto_tac)
+also have "... = `(\<not> ok \<and> ($tr \<le> $tr\<acute>)) \<or> ($wait \<and> ok' \<and> II\<^bsub>REL_VAR - OKAY\<^esub>) \<or> (\<not> $wait \<and> ok' \<and> $wait\<acute> \<and> (a \<notin> $ref\<acute>) \<and> ($tr \<le> $tr\<acute>)) \<or> (\<not> $wait \<and> ok' \<and> \<not> $wait\<acute> \<and> ($tr ^ \<langle>a\<rangle> = $tr\<acute>))`"  by(simp add:CondR_def, utp_pred_auto_tac)
+finally show ?thesis ..
+qed
+lemma Skip_form : "`SKIP`= `(\<not> ok \<and> ($tr \<le> $tr\<acute>)) \<or> ($wait \<and> ok' \<and> II\<^bsub>REL_VAR - OKAY\<^esub>) \<or> (\<not> $wait \<and> ok' \<and> (\<exists> ref .II\<^bsub>rea\<^esub>))`"by (utp_pred_auto_tac)
+lemma Chaos_form : "`CHAOS`= `(\<not> ok \<and> ($tr \<le> $tr\<acute>)) \<or> ($wait \<and> ok' \<and> II\<^bsub>REL_VAR - OKAY\<^esub> \<and> ($tr \<le> $tr\<acute>)) \<or> (\<not> $wait \<and> ($tr \<le> $tr\<acute>))`"by (utp_pred_auto_tac)
+
+lemma STOP_is_R1 : "R1 STOP = STOP "
+proof -
+have "`R1( STOP )` = `CSP1( ok' \<and> R1(\<delta>))`" by utp_pred_auto_tac
+thus ?thesis by(simp add:is_healthy_def \<delta>_is_R1 deadlock_def)
+qed
+
+lemma STOP_is_R2 : "R2 STOP = STOP" 
+proof - 
+have "`R2( STOP )` = `CSP1(R2( ok' \<and> \<delta>))`" by (simp add:deadlock_def CSP1_R2_commute)
+also have "... = `CSP1( ok' \<and> R2(\<delta>))`" by(simp add:R2_def R2s_def usubst typing defined closure, utp_pred_auto_tac)
+finally show ?thesis by (simp add:is_healthy_def \<delta>_is_R2 deadlock_def)
+qed
+
+lemma STOP_is_R3 : "R3 STOP = STOP" 
+proof - 
+have "`R3( STOP )` = `CSP1(R3( ok' \<and> \<delta>))`"by (simp add:deadlock_def CSP1_R3_commute)
+also have "... = `CSP1(ok' \<and> \<delta>)`" by utp_pred_auto_tac
+finally show ?thesis by (simp add:is_healthy_def deadlock_def)
+qed
+
+lemma STOP_is_CSP1 : "CSP1 STOP = STOP" by(simp add:deadlock_def CSP1_idempotent)
+
+lemma STOP_is_CSP2 : "CSP2 STOP = STOP" 
+proof -
+have "CSP2 STOP = `($okay\<acute> \<and> (II\<^bsub>rea\<^esub>[true/okay\<acute>] \<lhd> $wait \<rhd> (($tr = $tr\<acute>) \<and> $wait\<acute>))) \<or> (\<not> $okay \<and> ($tr \<le> $tr\<acute>))`"by(simp add:deadlock_def CSP2_form CSP1_def \<delta>_def R3_def usubst typing defined closure, utp_pred_auto_tac)
+also have "... = `CSP1(($okay\<acute> \<and> II\<^bsub>rea\<^esub>[true/okay\<acute>]) \<lhd> $wait \<rhd> ($okay\<acute> \<and> ($tr = $tr\<acute>) \<and> $wait\<acute>))`" by(simp add:CSP1_def, utp_pred_auto_tac)
+also have "... = `CSP1(($okay\<acute> \<and> II\<^bsub>rea\<^esub>) \<lhd> $wait \<rhd> ($okay\<acute> \<and> ($tr = $tr\<acute>) \<and> $wait\<acute>))`" by(metis aider3)
+also have "... = `CSP1($okay\<acute> \<and> (II\<^bsub>rea\<^esub> \<lhd> $wait \<rhd> (($tr = $tr\<acute>) \<and> $wait\<acute>)))`" by(utp_pred_auto_tac)
+finally show ?thesis by(simp add:deadlock_def \<delta>_def R3_def) 
+qed
+
+lemma Seq_comp_CSP : 
+  assumes "P is CSP \<and> Q is CSP"
+  shows "P;Q = `R(\<not>(P\<^sup>f\<^sub>f;R1(true)) \<and> \<not>(P\<^sup>t\<^sub>f;Q\<^sup>f\<^sub>f) \<turnstile> P\<^sup>t\<^sub>f;Q\<^sup>t)`"
+using assms
+proof -
+from assms have "P = `R(\<not> P\<^sup>f\<^sub>f \<turnstile> P\<^sup>t\<^sub>f)`" by(metis CSP_Closure)
+moreover from assms have "Q = `R(\<not> Q\<^sup>f\<^sub>f \<turnstile> Q\<^sup>t\<^sub>f)`" by(metis CSP_Closure)
+ultimately have "P;Q = `R(\<not> P\<^sup>f\<^sub>f \<turnstile> P\<^sup>t\<^sub>f);R(\<not> Q\<^sup>f\<^sub>f \<turnstile> Q\<^sup>t\<^sub>f)`" by metis
+thus ?thesis sorry qed
 
 lemma "`a \<rightarrow> SKIP` = `@a`"
-apply(simp add: prefixed_def )
+oops
+
+lemma L1 : "`CHAOS ; P` = `CHAOS`"
+sorry
+
+lemma L2 : "`STOP ; P` = `STOP`"
+sorry
 
 lemma L3 : "(P \<sqinter> Q) \<box> S = (P \<box> S) \<sqinter> (Q \<box> s)"
-
 oops
 
 lemma L4 : "P \<sqinter> (Q \<box> S) = (P \<sqinter> Q) \<box> (P \<sqinter> S)"
 oops
-
-lemma conj_through_dist_2 : "`P \<and> Q \<or> S` = `(P \<and> Q) \<or> (P \<and> S)`" sorry
-lemma negation_of_disjunction  : "`\<not>(P \<or> Q)` = `(\<not>P \<and> \<not>Q)`" sorry
-lemma \<delta>_and_SKIP_is_false : "`((ok\<acute> \<and> \<delta>) \<and> (\<not> ok \<and> ($tr \<le> $tr\<acute>)) \<and> SKIP) ; J\<^bsub>rea\<^esub> \<or> Q` = `Q`" sorry
-lemma aid : "`((\<not> ok \<and> ($tr \<le> $tr\<acute>)) \<and> (\<not> ok \<and> ($tr \<le> $tr\<acute>)) \<and> SKIP) ; J\<^bsub>rea\<^esub>` =`(\<not> ok \<and> ($tr \<le> $tr\<acute>))`" sorry
 
 lemma L5 : 
   assumes "P is CSP1" 
@@ -184,5 +240,4 @@ oops
 
 lemma L6sub : "`((a1\<rightarrow>P1) \<box> (a2\<rightarrow>P2)); Q` = `(a1\<rightarrow>(P1;Q)) \<box> (a2\<rightarrow>(P2;Q))`"
 oops
-
 end
