theories/theories/utp_reactive.thy
@@ -38,78 +38,112 @@ definition R1 :: " 'a WF_PREDICATE \<Rightarrow> 'a WF_PREDICATE" where
 
 text {* R2 ensures that the trace only gets longer *}
 
+definition R2s :: "'a WF_PREDICATE \<Rightarrow> 'a WF_PREDICATE" where
+"R2s(P) = `P[\<langle>\<rangle> / tr][($tr\<acute> - $tr) / tr\<acute>]`"
+
 definition R2 :: "'a WF_PREDICATE \<Rightarrow> 'a WF_PREDICATE" where
-"R2(P) = `P[\<langle>\<rangle> / tr][($tr\<acute> - $tr) / tr\<acute>]`"
+"R2(P) = R1 (R2s P)"
 
 definition R3 :: "'a WF_PREDICATE \<Rightarrow> 'a WF_PREDICATE" where
 "R3(P) = `II\<^bsub>rea\<^esub> \<lhd> $wait \<rhd> P`"
 
+definition R :: "'a WF_PREDICATE \<Rightarrow> 'a WF_PREDICATE" where 
+"R P = (R1 \<circ> R2 \<circ> R3)P"
+
 syntax 
   "_upred_R1" :: "upred \<Rightarrow> upred" ("R1'(_')")
   "_upred_R2" :: "upred \<Rightarrow> upred" ("R2'(_')")
+  "_upred_R2s" :: "upred \<Rightarrow> upred" ("R2s'(_')")
   "_upred_R3" :: "upred \<Rightarrow> upred" ("R3'(_')")
+  "_upred_R" :: "upred \<Rightarrow> upred" ("R'(_')")
 
 translations
   "_upred_R1 P" == "CONST R1 P"
   "_upred_R2 P" == "CONST R2 P"
+  "_upred_R2s P" == "CONST R2s P"
   "_upred_R3 P" == "CONST R3 P"
+  "_upred_R P" == "CONST R P"
 
 declare R1_def [eval, evalr, evalrr, evalrx]
 declare R2_def [eval, evalr, evalrr, evalrx]
+declare R2s_def [eval, evalr, evalrr, evalrx]
 declare R3_def [eval, evalr, evalrr, evalrx]
 declare is_healthy_def [eval, evalr, evalrr, evalrx]
 declare SkipREA_def [eval, evalr, evalrr, evalrx]
+declare R_def [eval, evalr, evalrr, evalrx]
+
+thm SkipRA_unfold [of "tr\<down>"]
+
+lemma Skip_is_R2s : "`R2s(II\<^bsub>REL_VAR - {okay\<down>, okay\<down>\<acute>}\<^esub>)` = `II\<^bsub>REL_VAR - {okay\<down>, okay\<down>\<acute>}\<^esub>`"sorry
+lemma Skip_is_R1 : "`R1(II\<^bsub>REL_VAR - {okay\<down>, okay\<down>\<acute>}\<^esub>)` = `II\<^bsub>REL_VAR - {okay\<down>, okay\<down>\<acute>}\<^esub>`"sorry
+lemma tr_conserved_is_R2 : "`R2s($tr = $tr\<acute>)` = `($tr = $tr\<acute>)`"apply(simp add:R2s_def usubst typing defined closure, utp_pred_auto_tac)sorry
+lemma helper1 : "`$wait \<and> II\<^bsub>REL_VAR - {okay\<down>, okay\<down>\<acute>}\<^esub>` = `$wait \<and> $wait\<acute> \<and> II\<^bsub>REL_VAR - {okay\<down>, okay\<down>\<acute>}\<^esub>`"sorry
+lemma helper2 : "`($wait\<acute> \<and> Q) ; R3(P)` = `$wait\<acute> \<and> Q`"sorry
+lemma helper3 : "`(\<not> ok \<and> $wait \<and> ($tr \<le> $tr\<acute>)) ; P` = `(\<not> ok \<and> $wait \<and> ($tr \<le> $tr\<acute>))`"sorry
+lemma helper4 : "`\<langle>\<rangle> = ($tr\<acute> - $tr)` =`$tr\<acute> = $tr`"sorry
+lemma wait_then_P_equals_wait : "`(($wait \<and> II\<^bsub>rea\<^esub>) \<and> ($tr \<le> $tr\<acute>)) ; P` = `(($wait \<and> II\<^bsub>rea\<^esub>) \<and> ($tr \<le> $tr\<acute>))`" sorry
+lemma R2s_R3_commute : "R2s (R3 P) = R3 (R2s P)" sorry
+lemma Assist : "`P[false/okay\<acute>] \<or> P[true/okay\<acute>]` = `P`"sorry
+lemma Assist7 : "`(($tr < $tr\<acute>) \<and> ($tr^\<langle>a\<rangle> =$tr\<acute>))` = `($tr^\<langle>a\<rangle> =$tr\<acute>)`" sorry
+
+lemma tr_conserved_is_R1 : "`R1($tr = $tr\<acute>)` = `($tr = $tr\<acute>)`" by (simp add:R1_def, utp_pred_auto_tac)
+lemma R2s_idempotent : "`R2s(R2s(P))` = `R2s(P)`"by(simp add:R2s_def, simp add:usubst typing closure defined unrest)
+lemma SkipREA_is_R1: "`R1(II\<^bsub>rea\<^esub>)`= `II\<^bsub>rea\<^esub>`"
+proof-
+have "`R1(II\<^bsub>rea\<^esub>)`=`(\<not> $okay \<and> ($tr \<le> $tr\<acute>)) \<or>($okay\<acute> \<and> R1(II\<^bsub>REL_VAR - {okay\<down>, okay\<down>\<acute>}\<^esub>))`" by(simp add:R1_def SkipREA_def, utp_pred_auto_tac)
+thus ?thesis by (simp add:Skip_is_R1 SkipREA_def)
+qed
+lemma SkipREA_is_R2 : "`R2(II\<^bsub>rea\<^esub>)` = `II\<^bsub>rea\<^esub>`"
+proof-
+have "`R2(II\<^bsub>rea\<^esub>)` = `(\<not> $okay \<and> ($tr \<le> $tr\<acute>)) \<or>($okay\<acute> \<and> R1(R2s(II\<^bsub>REL_VAR - {okay\<down>, okay\<down>\<acute>}\<^esub>)))`" by(simp add: R2_def R1_def SkipREA_def R2s_def usubst typing defined closure, utp_pred_auto_tac)
+thus ?thesis by (simp add:Skip_is_R2s Skip_is_R1 SkipREA_def)
+qed
+lemma wait_is_R2s : "`R2s($wait)` = `$wait`" by(simp add:R2s_def usubst closure typing defined)
+lemma R2s_destroys_R1 : "R2s (R1 P) = R2s P" by(simp add:R2s_def R1_def usubst closure typing defined, utp_pred_auto_tac)
+lemma conj_distributes_through_conditional : "`(P \<lhd> b \<rhd> Q) \<and> S` = `(P \<and> S)\<lhd> b \<rhd>(Q \<and> S)`"by utp_pred_auto_tac
+lemma R2s_distributes_through_conjunction : "`R2s(P \<and> Q)` = `R2s(P) \<and> R2s(Q)`" by utp_pred_auto_tac
+lemma R2s_distributes_through_conditional : "`R2s(P \<lhd> b \<rhd> Q)` = `R2s(P)\<lhd> R2s(b) \<rhd>R2s(Q)`"by utp_pred_auto_tac
+lemma R2_distributes_through_conditional : "`R2(P \<lhd> b \<rhd> Q)` =`R2(P) \<lhd> R2s(b) \<rhd> R2(Q)`" by utp_pred_auto_tac
+lemma R3_distributes_through_disjunction :"`R3(P \<or> Q)` = `R3(P) \<or> R3(Q)`"by utp_pred_auto_tac
+lemma R3_distributes_through_conditional :"`R3(P \<lhd> b \<rhd> Q)` = `R3(P) \<lhd> R3(b) \<rhd> R3(Q)`"by utp_pred_auto_tac
+lemma seq_comp_assoc : "`(P ; Q) ; S` = `P ; (Q ; S)`"by (metis SemiR_assoc)
+lemma R2s_distributes_through_disjunction: "`R2s(A \<or> C)` = `R2s(A) \<or> R2s(C)`" by utp_pred_auto_tac
+lemma R1_not_ok : "`(\<not> ok \<and> ($tr \<le> $tr\<acute>))` = `R1(\<not> ok)`" by (simp add:R1_def)
+lemma not_ok_is_R2s : "`R2s(\<not> ok)` = `\<not> ok`" by (simp add:R2s_def usubst typing defined closure) 
+lemma ok_dash_is_R2s : "`R2s(ok')` = `ok'`"by (simp add:R2s_def usubst typing defined closure)
+lemma Assist5 : "`R1(P \<and> Q)` = `P \<and> R1(Q)`" by utp_pred_auto_tac
+lemma wait_is_R2 : "`$wait[($tr\<acute> - $tr)/tr\<acute>][\<langle>\<rangle>/tr]` = `$wait`" by(simp add:usubst typing defined closure)
+lemma not_wait_is_R2 : "`(\<not> $wait)[($tr\<acute> - $tr)/tr\<acute>][\<langle>\<rangle>/tr]` = `\<not> $wait`" by(simp add:usubst typing defined closure)
+lemma conj_through_dist_2 : "`P \<and> Q \<or> S` = `(P \<and> Q) \<or> (P \<and> S)`" by utp_pred_auto_tac
+lemma negation_of_disjunction  : "`\<not>(P \<or> Q)` = `(\<not>P \<and> \<not>Q)`" by utp_pred_auto_tac
+lemma DesignD_form : "`(P \<turnstile> Q)` = `\<not>ok \<or> \<not>P \<or> (ok' \<and> Q)`" by(simp add:DesignD_def, utp_pred_auto_tac)
+lemma aider3 : "`$okay\<acute> \<and> II\<^bsub>rea\<^esub>[true/okay\<acute>]` = `$okay\<acute> \<and> II\<^bsub>rea\<^esub>`"by(simp add:SkipREA_def usubst typing defined closure, utp_pred_auto_tac)
 
 lemma R1_idempotent : "`R1(R1(P))` = `R1(P)`" by (utp_rel_tac)
-
-
-lemma R2_idempotent : "`R2(R2(P))` = `R2(P)`"
-  by (simp add:R2_def, simp add:usubst typing closure defined unrest)
-
+lemma R2_idempotent : "`R2(R2(P))` = `R2(P)`" by(simp add:R2_def R2s_destroys_R1 R2s_idempotent)
 lemma R3_idempotent : "`R3(R3(P))` = `R3(P)`" by (utp_pred_auto_tac)
 
-lemma R1_monotonic : "[P \<Rightarrow> Q] \<Longrightarrow> [R1(P) \<Rightarrow> R1(Q)]" by(utp_pred_tac)
-lemma R2_monotonic : "[P \<Rightarrow> Q] \<Longrightarrow> [R2(P) \<Rightarrow> R2(Q)]" by(utp_pred_tac)
-lemma R3_monotonic : "[P \<Rightarrow> Q] \<Longrightarrow> [R3(P) \<Rightarrow> R3(Q)]" by(utp_pred_tac)
+lemma R1_monotonic : "[P \<Rightarrow> Q] \<Longrightarrow> [R1(P) \<Rightarrow> R1(Q)]" by utp_pred_tac
+lemma R2_monotonic : "[P \<Rightarrow> Q] \<Longrightarrow> [R2(P) \<Rightarrow> R2(Q)]" by utp_pred_tac
+lemma R3_monotonic : "[P \<Rightarrow> Q] \<Longrightarrow> [R3(P) \<Rightarrow> R3(Q)]" by utp_pred_tac
 
-lemma SkipREA_is_R1: "`II\<^bsub>rea\<^esub> \<and> ($tr \<le> $tr\<acute>)`= `II\<^bsub>rea\<^esub>`" 
-  by (auto simp add:eval closure typing defined)
-
-lemma R1_true_is_R2 : "`($tr \<le> $tr\<acute>)[($tr\<acute> - $tr)/tr\<acute>][\<langle>\<rangle>/tr]` = `($tr \<le> $tr\<acute>)`" sorry
-lemma SkipREA_is_R2 : "`II\<^bsub>rea\<^esub>[($tr\<acute> - $tr)/tr\<acute>][\<langle>\<rangle>/tr]` = `II\<^bsub>rea\<^esub>`" sorry
-lemma wait_is_R2 : "`$wait[($tr\<acute> - $tr)/tr\<acute>][\<langle>\<rangle>/tr]` = `$wait`" sorry
+lemma R1_R2_commute : "R1 (R2 P) = R2 (R1 P)" by (simp add:R2_def R1_idempotent R2s_destroys_R1)
 
 lemma R1_R3_commute : "R1 (R3 P) = R3 (R1 P)" 
 proof - 
-  have "R1 (R3 P) = `(II\<^bsub>rea\<^esub> \<lhd> $wait \<rhd> P) \<and> ($tr \<le> $tr\<acute>)`" by (utp_rel_tac)
-  also have "... = `(II\<^bsub>rea\<^esub> \<and> ($tr \<le> $tr\<acute>)) \<lhd> $wait \<rhd> (P \<and> ($tr \<le> $tr\<acute>))`" by (utp_pred_auto_tac)
-  ultimately show ?thesis by (simp add:SkipREA_is_R1, utp_rel_tac)
-qed
-
-lemma R1_R2_commute : "R1 (R2 P) = R2 (R1 P)" 
-proof -
-  have "R2 (R1 P) = `(P \<and> ($tr \<le> $tr\<acute>))[\<langle>\<rangle>/tr][($tr\<acute> - $tr)/tr\<acute>]`" by (utp_rel_tac)
-  also have "... = `P[\<langle>\<rangle>/tr][($tr\<acute> - $tr)/tr\<acute>] \<and> ($tr \<le> $tr\<acute>)`" 
-    sorry(*by (simp add:usubst erasure typing defined closure R1_true_is_R2)*)
-  ultimately show ?thesis by (utp_rel_tac)
+  have "R1 (R3 P) = `(II\<^bsub>rea\<^esub> \<lhd> $wait \<rhd> P) \<and> ($tr \<le> $tr\<acute>)`" by utp_rel_tac
+  also have "... = `(II\<^bsub>rea\<^esub> \<and> ($tr \<le> $tr\<acute>)) \<lhd> $wait \<rhd> (P \<and> ($tr \<le> $tr\<acute>))`" by utp_pred_auto_tac
+  also have "... = `II\<^bsub>rea\<^esub> \<lhd> $wait \<rhd> (P \<and> ($tr \<le> $tr\<acute>))`" by (metis R1_def SkipREA_is_R1)
+  ultimately show ?thesis by utp_pred_auto_tac
 qed
 
 lemma R2_R3_commute : "R2 (R3 P) = R3 (R2 P)" 
 proof - 
-  have "R2 (R3 P) = `(II\<^bsub>rea\<^esub> \<lhd> $wait \<rhd> P)[\<langle>\<rangle>/tr][($tr\<acute> - $tr)/tr\<acute>]`" by (utp_rel_tac)
-  also have "... = `II\<^bsub>rea\<^esub> \<lhd> $wait \<rhd> (P[\<langle>\<rangle>/tr][($tr\<acute> - $tr)/tr\<acute>])`"sorry(* by (simp add:usubst erasure typing defined closure SkipREA_is_R2 wait_is_R2)*)
-  ultimately show ?thesis by (utp_rel_tac)
+  have "R2 (R3 P) = `R2(II\<^bsub>rea\<^esub>) \<lhd> R2s($wait) \<rhd> R2(P)`" by (simp add:R3_def R2_distributes_through_conditional)
+  also have "... = `II\<^bsub>rea\<^esub> \<lhd> $wait \<rhd> R2(P)`" by(simp add: SkipREA_is_R2, simp add:R2s_def usubst closure typing defined)
+  ultimately show ?thesis by utp_pred_tac
 qed
 
-definition R :: "'a WF_PREDICATE \<Rightarrow> 'a WF_PREDICATE" where 
-"R P = (R1 \<circ> R2 \<circ> R3)P"
-
-declare R_def [eval, evalr, evalrr, evalrx]
-syntax 
-  "_upred_R" :: "upred \<Rightarrow> upred" ("R'(_')")
-
-translations
-  "_upred_R P" == "CONST R P"
 
 lemma SkipREA_CondR_SkipR: 
   "`II\<^bsub>rea\<^esub>` = `II \<lhd> ok \<rhd> ($tr \<le> $tr\<acute>)`"
